Examples/EdmondsKarp_Maxflow/EdmondsKarp_Time.thy
@@ -56,7 +56,24 @@ lemma"(\<lambda>x. real ((57 +
 
 lemma rbt_i_408: "rbt_insert_logN 1 = 408" unfolding rbt_insert_logN_def rbt_insert_time_def rbt_absch_def rbt_ins_time_def by simp
 
-lemma "edka_cost \<in> \<Theta>\<^sub>2(\<lambda>(V::nat,E::nat).  real V * real E * real V * real E + real V * real E * real V * ln V)"
+
+
+
+
+lemma "(\<lambda>x::nat. real ((3 ))) \<in> \<Theta>(\<lambda>(x). real 1)" 
+  by auto2
+definition f :: "nat \<Rightarrow> nat" where "f x = x"
+lemma "(\<lambda>x::nat. real (( f 23 ))) \<in> \<Theta>(\<lambda>(x). real 1)" 
+  by auto2
+
+lemma "(\<lambda>x. real ((32 ))) \<in> \<Theta>\<^sub>2(\<lambda>(V::nat,E::nat). 1)" 
+  apply (subst surjective_pairing) by auto2
+
+lemma "(\<lambda>x. real ((rbt_insert_logN 1 ))) \<in> \<Theta>\<^sub>2(\<lambda>(V::nat,E::nat). 1)" 
+  apply (subst surjective_pairing) by auto2
+
+
+lemma "edka_cost \<in> \<Theta>\<^sub>2(\<lambda>(V::nat,E::nat). V * E * E * V + V * E * V * ln V)"
   apply (subst surjective_pairing)
   unfolding edka_cost_simp rbt_i_408 by(auto2)
   
